Rename conn -> rpc.

store/impl.v
@@ -5,7 +5,7 @@ From iris.algebra Require Import agree auth csum gset gmap excl frac.
 From iris.algebra Require Import max_prefix_list.
 From iris.heap_lang Require Import notation proofmode.
 From iris.heap_lang.lib Require Import lock ticket_lock.
-From cryptis Require Import lib term cryptis primitives tactics conn.
+From cryptis Require Import lib term cryptis primitives tactics rpc.
 From cryptis.store Require Import alist db.
 
 Set Implicit Arguments.
@@ -21,29 +21,29 @@ Section Client.
 Variable N : namespace.
 
 Definition connect : val := λ: "c" "skA" "vkB",
-  Conn.connect N "c" "skA" "vkB".
+  RPC.connect N "c" "skA" "vkB".
 
 Definition store : val := λ: "c" "cs" "k" "v",
-  Conn.write (N.@"store") "c" "cs" ["k"; "v"];;
-  Conn.read (N.@"ack_store") "c" "cs";;
-  Conn.tick "cs".
+  RPC.write (N.@"store") "c" "cs" ["k"; "v"];;
+  RPC.read (N.@"ack_store") "c" "cs";;
+  RPC.tick "cs".
 
 Definition load : val := λ: "c" "cs" "k",
-  Conn.write (N.@"load") "c" "cs" ["k"];;
-  let: "ts" := Conn.read (N.@"ack_load") "c" "cs" in
-  Conn.tick "cs";;
+  RPC.write (N.@"load") "c" "cs" ["k"];;
+  let: "ts" := RPC.read (N.@"ack_load") "c" "cs" in
+  RPC.tick "cs";;
   match: "ts" with
     NONE => TInt 0
   | SOME "ts" => Fst "ts"
   end.
 
 Definition create : val := λ: "c" "cs" "k" "v",
-  Conn.write (N.@"create") "c" "cs" ["k"; "v"];;
-  Conn.read (N.@"ack_create") "c" "cs";;
-  Conn.tick "cs".
+  RPC.write (N.@"create") "c" "cs" ["k"; "v"];;
+  RPC.read (N.@"ack_create") "c" "cs";;
+  RPC.tick "cs".
 
 Definition close : val := λ: "c" "cs",
-  Conn.close N "c" "cs".
+  RPC.close N "c" "cs".
 
 End Client.
 
@@ -61,8 +61,8 @@ Definition handle_store N : val :=
 λ: "c" "cs" "db" "req",
   list_match: ["k"; "v"] := "req" in
   SAList.insert "db" "k" "v";;
-  Conn.write (N.@"ack_store") "c" "cs" [];;
-  Conn.tick "cs";;
+  RPC.write (N.@"ack_store") "c" "cs" [];;
+  RPC.tick "cs";;
   SOME #true.
 
 (* FIXME: Should return an error when the key is not present *)
@@ -70,8 +70,8 @@ Definition handle_load N : val :=
 λ: "c" "cs" "db" "req",
   list_match: ["k"] := "req" in
   bind: "data" := SAList.find "db" "k" in
-  Conn.write (N.@"ack_load") "c" "cs" ["data"];;
-  Conn.tick "cs";;
+  RPC.write (N.@"ack_load") "c" "cs" ["data"];;
+  RPC.tick "cs";;
   SOME #true.
 
 Definition handle_create N : val :=
@@ -85,8 +85,8 @@ Definition handle_create N : val :=
       #1
     end in
   let: "m" := ["k"; "v"; tint "success"] in
-  Conn.write (N.@"ack_create") "c" "cs" "m";;
-  Conn.tick "cs";;
+  RPC.write (N.@"ack_create") "c" "cs" "m";;
+  RPC.tick "cs";;
   SOME #true.
 
 Definition conn_handler N : val :=
@@ -95,7 +95,7 @@ Definition conn_handler N : val :=
     (N.@"load", handle_load N "c" "cs" "db");
     (N.@"create", handle_create N "c" "cs" "db")
   ] in λ: "c" "cs" "db" "lock",
-     Conn.handle N "c" "cs" handlers;;
+     RPC.handle N "c" "cs" handlers;;
      lock.release "lock".
 
 Definition find_client : val := λ: "ss" "client_key",
@@ -112,13 +112,13 @@ Definition find_client : val := λ: "ss" "client_key",
 Definition listen N : val := λ: "c" "ss",
   let: "secret_key" := Fst "ss" in
   let: "clients" := Snd "ss" in
-  let: "res" := Conn.listen "c" in
+  let: "res" := RPC.listen "c" in
   let: "client_key" := Snd "res" in
   let: "account" := find_client "ss" "client_key" in
   let: "db" := Fst "account" in
   let: "lock" := Snd "account" in
   acquire "lock";;
-  let: "cs" := Conn.confirm N "c" "secret_key" "res" in
+  let: "cs" := RPC.confirm N "c" "secret_key" "res" in
   Fork (conn_handler N "c" "cs" "db" "lock").
 
 End Server.
