rpc.v
@@ -1,0 +1,12 @@
+From cryptis Require Import iso_dh.
+From cryptis.rpc Require Import props impl proofs.
+
+Module RPC.
+
+Include Props.
+Include Impl.
+Include Proofs.
+
+End RPC.
+
+Coercion RPC.cs_si : RPC.state >-> sess_info.
