store/server_proofs.v
@@ -6,7 +6,7 @@ From iris.algebra Require Import max_prefix_list.
 From iris.heap_lang Require Import notation proofmode.
 From iris.heap_lang.lib Require Import ticket_lock.
 From cryptis Require Import lib term cryptis primitives tactics.
-From cryptis Require Import gmeta nown role iso_dh conn.
+From cryptis Require Import gmeta nown role iso_dh rpc.
 From cryptis.store Require Import impl shared alist db.
 From cryptis.store.server_proofs Require Import load store create.
 
@@ -23,7 +23,7 @@ Notation iProp := (iProp Σ).
 
 Context `{!storeGS Σ}.
 
-Implicit Types (cs : Conn.state).
+Implicit Types (cs : RPC.state).
 Implicit Types skI skR kS t : term.
 Implicit Types n : nat.
 Implicit Types γ : gname.
@@ -52,7 +52,7 @@ move=> kI _. solve_ndisj.
 Qed.
 
 (* Lemma wp_server_conn_handler_body c skI skR cs n vdb : *)
-(*   Conn.cs_role cs = Resp → *)
+(*   RPC.cs_role cs = Resp → *)
 (*   channel c -∗ *)
 (*   store_ctx N -∗ *)
 (*   {{{ server_db_connected N skI skR cs n vdb }}} *)
@@ -61,10 +61,10 @@ Qed.
 (* Proof. *)
 (* iIntros "% #chan_c #ctx !> %Φ (conn & db) post". *)
 (* wp_lam. wp_pures. *)
-(* rewrite !Conn.subst_select /=. *)
+(* rewrite !RPC.subst_select /=. *)
 (* iApply (wp_wand with "[conn db] post"). *)
 (* iRevert "db". *)
-(* iApply Conn.wp_select => //=; do !iSplitR => //. *)
+(* iApply RPC.wp_select => //=; do !iSplitR => //. *)
 (* - by iApply wp_server_handle_store. *)
 (* - by iApply wp_server_handle_load. *)
 (* - by iApply wp_server_handle_create. *)
@@ -72,7 +72,7 @@ Qed.
 (* Qed. *)
 
 Lemma wp_server_conn_handler c cs n vdb vlock γlock :
-  Conn.cs_role cs = Resp →
+  RPC.cs_role cs = Resp →
   channel c -∗
   is_lock γlock vlock (server_db_disconnected N (si_init cs) (si_resp cs) vdb) -∗
   store_ctx N -∗
@@ -83,9 +83,9 @@ Lemma wp_server_conn_handler c cs n vdb vlock γlock :
 Proof.
 iIntros "% #chan_c #lock #ctx".
 iIntros "!> %Φ ((conn & token & db) & locked) post".
-wp_lam. wp_pures. rewrite !Conn.subst_handle /=.
+wp_lam. wp_pures. rewrite !RPC.subst_handle /=.
 iPoseProof (store_ctx_conn_ctx with "ctx") as "?".
-wp_apply (Conn.wp_handle with "[//] [//] [] conn token db");
+wp_apply (RPC.wp_handle with "[//] [//] [] conn token db");
   first (rewrite /=; do !iSplitR => //).
 - iApply wp_server_handle_store => //.
 - iApply wp_server_handle_load => //.
@@ -95,7 +95,7 @@ wp_pures.
 wp_apply (release_spec with "[$locked dis vdb]") => //.
 iSplit => //. iExists n'. iFrame.
 iSplit => //. iDestruct "db_at" as "[fail|db_at]"; eauto.
-iLeft. by iApply Conn.session_failed_failure.
+iLeft. by iApply RPC.session_failed_failure.
 Qed.
 
 Lemma wp_server_find_client ss skI :
@@ -168,7 +168,7 @@ Proof.
 iIntros "%Φ (#? & #chan_c & #ctx & server) post".
 wp_lam; wp_pures.
 iPoseProof (store_ctx_conn_ctx with "ctx") as "?".
-wp_apply (Conn.wp_listen
+wp_apply (RPC.wp_listen
          with "[# //] [# //] [# //] [#]") => //;
   try by solve_ndisj.
 iIntros "%ga %skA #[p_ga p_skA]". wp_pures.
@@ -184,7 +184,7 @@ iDestruct "dis" as "(%n & dis & %db & #p_db & vdb & #db_at)".
 iAssert (sign_key (ss_key ss)) as "#?".
 { by iDestruct "server" as "(% & % & ? & _)". }
 wp_pures.
-wp_apply (Conn.wp_confirm with "[] [] [] [$dis]") => //.
+wp_apply (RPC.wp_confirm with "[] [] [] [$dis]") => //.
 { do 3!iSplit => //. }
 iIntros "%cs {db_at} (%e_rl & <- & <- & conn & #db_at & token)".
 wp_pures.
